Weidenbach_Book/IsaSAT/IsaSAT_VMTF.thy
@@ -505,7 +505,7 @@ definition (in -) atoms_hash_set_member where
 
 
 definition isa_vmtf_mark_to_rescore
-  :: \<open>nat \<Rightarrow> isa_vmtf_remove_int \<Rightarrow> isa_vmtf_remove_int\<close>
+  :: \<open>nat \<Rightarrow> bump_heuristics \<Rightarrow> bump_heuristics\<close>
 where
   \<open>isa_vmtf_mark_to_rescore L = (\<lambda>((ns, m, fst_As, next_search), to_remove).
      ((ns, m, fst_As, next_search), atoms_hash_insert L to_remove))\<close>
@@ -522,7 +522,7 @@ lemma isa_vmtf_mark_to_rescore_vmtf_mark_to_rescore:
   by (intro frefI nres_relI)
     (auto intro!: atoms_hash_del_op_set_insert[THEN fref_to_Down_unRET_uncurry])
 
-definition (in -) isa_vmtf_unset :: \<open>nat \<Rightarrow> isa_vmtf_remove_int \<Rightarrow> isa_vmtf_remove_int\<close> where
+definition (in -) isa_vmtf_unset :: \<open>nat \<Rightarrow> bump_heuristics \<Rightarrow> bump_heuristics\<close> where
 \<open>isa_vmtf_unset = (\<lambda>L ((ns, m, fst_As, lst_As, next_search), to_remove).
   (if next_search = None \<or> stamp (ns ! (the next_search)) < stamp (ns ! L)
   then ((ns, m, fst_As, lst_As, Some L), to_remove)
@@ -542,7 +542,7 @@ lemma vmtf_unset_pre_vmtf:
 
 lemma vmtf_unset_pre:
   assumes
-    \<open>((ns, m, fst_As, lst_As, next_search), to_remove) \<in> isa_vmtf \<A> M\<close> and
+    \<open>((ns, m, fst_As, lst_As, next_search), to_remove) \<in> bump_heur \<A> M\<close> and
     \<open>L \<in># \<A>\<close>
   shows \<open>vmtf_unset_pre L ((ns, m, fst_As, lst_As, next_search), to_remove)\<close>
   using assms vmtf_unset_pre_vmtf[of ns m fst_As lst_As next_search _ \<A> M L]
@@ -551,13 +551,13 @@ lemma vmtf_unset_pre:
 
 lemma vmtf_unset_pre':
   assumes
-    \<open>vm \<in> isa_vmtf \<A> M\<close> and
+    \<open>vm \<in> bump_heur \<A> M\<close> and
     \<open>L \<in># \<A>\<close>
   shows \<open>vmtf_unset_pre L vm\<close>
   using assms by (cases vm) (auto dest: vmtf_unset_pre)
 
 (*
-definition isa_vmtf_mark_to_rescore_and_unset :: \<open>nat \<Rightarrow> isa_vmtf_remove_int \<Rightarrow> isa_vmtf_remove_int\<close>
+definition isa_vmtf_mark_to_rescore_and_unset :: \<open>nat \<Rightarrow> bump_heuristics \<Rightarrow> bump_heuristics\<close>
 where
   \<open>isa_vmtf_mark_to_rescore_and_unset L M = isa_vmtf_mark_to_rescore L (isa_vmtf_unset L M)\<close>
 
@@ -589,8 +589,8 @@ lemma isa_vmtf_unset_vmtf_unset:
   by (intro frefI nres_relI) auto
 
 lemma isa_vmtf_unset_isa_vmtf:
-  assumes \<open>vm \<in> isa_vmtf \<A> M\<close> and \<open>L \<in># \<A>\<close>
-  shows \<open>isa_vmtf_unset L vm \<in> isa_vmtf \<A> M\<close>
+  assumes \<open>vm \<in> bump_heur \<A> M\<close> and \<open>L \<in># \<A>\<close>
+  shows \<open>isa_vmtf_unset L vm \<in> bump_heur \<A> M\<close>
 proof -
   obtain vm0 to_remove to_remove' where
     vm: \<open>vm = (vm0, to_remove)\<close> and
@@ -607,9 +607,9 @@ proof -
 qed
 
 lemma isa_vmtf_tl_isa_vmtf:
-  assumes \<open>vm \<in> isa_vmtf \<A> M\<close> and \<open>M \<noteq> []\<close> and \<open>lit_of (hd M) \<in># \<L>\<^sub>a\<^sub>l\<^sub>l \<A>\<close> and
+  assumes \<open>vm \<in> bump_heur \<A> M\<close> and \<open>M \<noteq> []\<close> and \<open>lit_of (hd M) \<in># \<L>\<^sub>a\<^sub>l\<^sub>l \<A>\<close> and
     \<open>L = (atm_of (lit_of (hd M)))\<close>
-  shows \<open>isa_vmtf_unset L vm \<in> isa_vmtf \<A> (tl M)\<close>
+  shows \<open>isa_vmtf_unset L vm \<in> bump_heur \<A> (tl M)\<close>
 proof -
   let ?L = \<open>atm_of (lit_of (hd M))\<close>
   obtain vm0 to_remove to_remove' where
@@ -629,7 +629,7 @@ qed
 
 
 
-definition isa_vmtf_find_next_undef :: \<open>isa_vmtf_remove_int \<Rightarrow> trail_pol \<Rightarrow> (nat option) nres\<close> where
+definition isa_vmtf_find_next_undef :: \<open>bump_heuristics \<Rightarrow> trail_pol \<Rightarrow> (nat option) nres\<close> where
 \<open>isa_vmtf_find_next_undef = (\<lambda>((ns, m, fst_As, lst_As, next_search), to_remove) M. do {
     WHILE\<^sub>T\<^bsup>\<lambda>next_search. next_search \<noteq> None \<longrightarrow> defined_atm_pol_pre M (the next_search)\<^esup>
       (\<lambda>next_search. next_search \<noteq> None \<and> defined_atm_pol M (the next_search))
@@ -691,8 +691,8 @@ where
 find_theorems isa_vmtf_mark_to_rescore
 
 definition isa_vmtf_rescore_body
- :: \<open>nat clause_l \<Rightarrow> trail_pol \<Rightarrow> isa_vmtf_remove_int \<Rightarrow>
-    (nat \<times> isa_vmtf_remove_int) nres\<close>
+ :: \<open>nat clause_l \<Rightarrow> trail_pol \<Rightarrow> bump_heuristics \<Rightarrow>
+    (nat \<times> bump_heuristics) nres\<close>
 where
   \<open>isa_vmtf_rescore_body C _ vm = do {
          WHILE\<^sub>T\<^bsup>\<lambda>(i, vm). i \<le> length C  \<and>
@@ -708,8 +708,8 @@ where
     }\<close>
 
 definition isa_vmtf_rescore
- :: \<open>nat clause_l \<Rightarrow> trail_pol \<Rightarrow> isa_vmtf_remove_int \<Rightarrow>
-       (isa_vmtf_remove_int) nres\<close>
+ :: \<open>nat clause_l \<Rightarrow> trail_pol \<Rightarrow> bump_heuristics \<Rightarrow>
+       (bump_heuristics) nres\<close>
 where
   \<open>isa_vmtf_rescore C M vm = do {
       (_, vm) \<leftarrow> isa_vmtf_rescore_body C M vm;
@@ -1107,394 +1107,6 @@ lemma vmtf_mark_to_rescore_also_reasons_cl_spec:
         (auto simp: arena_lifting arena_lifting_list image_image uminus_\<A>\<^sub>i\<^sub>n_iff)
     done
   done
-
-
-
-section \<open>Backtrack level for Restarts\<close>
-
-text \<open>
-  We here find out how many decisions can be reused. Remark that since VMTF does not reuse many levels anyway,
-  the implementation might be mostly useless, but I was not aware of that when I implemented it.
-\<close>
-(* TODO ded-uplicate definitions *)
-definition find_decomp_w_ns_pre where
-  \<open>find_decomp_w_ns_pre \<A> = (\<lambda>((M, highest), vm).
-       no_dup M \<and>
-       highest < count_decided M \<and>
-       isasat_input_bounded \<A> \<and>
-       literals_are_in_\<L>\<^sub>i\<^sub>n_trail \<A> M \<and>
-       vm \<in> vmtf \<A> M)\<close>
-
-definition find_decomp_wl_imp
-  :: \<open>nat multiset \<Rightarrow> (nat, nat) ann_lits \<Rightarrow> nat \<Rightarrow> vmtf_remove_int \<Rightarrow>
-       ((nat, nat) ann_lits \<times> vmtf_remove_int) nres\<close>
-where
-  \<open>find_decomp_wl_imp \<A> = (\<lambda>M\<^sub>0 lev vm. do {
-    let k = count_decided M\<^sub>0;
-    let M\<^sub>0 = trail_conv_to_no_CS M\<^sub>0;
-    let n = length M\<^sub>0;
-    pos \<leftarrow> get_pos_of_level_in_trail M\<^sub>0 lev;
-    ASSERT((n - pos) \<le> uint32_max);
-    ASSERT(n \<ge> pos);
-    let target = n - pos;
-    (_, M, vm') \<leftarrow>
-       WHILE\<^sub>T\<^bsup>\<lambda>(j, M, vm'). j \<le> target \<and>
-           M = drop j M\<^sub>0 \<and> target \<le> length M\<^sub>0 \<and>
-           vm' \<in> vmtf \<A> M \<and> literals_are_in_\<L>\<^sub>i\<^sub>n \<A> (lit_of `# mset M)\<^esup>
-         (\<lambda>(j, M, vm). j < target)
-         (\<lambda>(j, M, vm). do {
-            ASSERT(M \<noteq> []);
-            ASSERT(Suc j \<le> uint32_max);
-            let L = atm_of (lit_of_hd_trail M);
-            ASSERT(L \<in># \<A>);
-            RETURN (j + 1, tl M, vmtf_unset L vm)
-         })
-         (0, M\<^sub>0, vm);
-    ASSERT(lev = count_decided M);
-    let M = trail_conv_back lev M;
-    RETURN (M, vm')
-  })\<close>
-
-definition isa_find_decomp_wl_imp
-  :: \<open>trail_pol \<Rightarrow> nat \<Rightarrow> isa_vmtf_remove_int \<Rightarrow> (trail_pol \<times> isa_vmtf_remove_int) nres\<close>
-where
-  \<open>isa_find_decomp_wl_imp = (\<lambda>M\<^sub>0 lev vm. do {
-    let k = count_decided_pol M\<^sub>0;
-    let M\<^sub>0 = trail_pol_conv_to_no_CS M\<^sub>0;
-    ASSERT(isa_length_trail_pre M\<^sub>0);
-    let n = isa_length_trail M\<^sub>0;
-    pos \<leftarrow> get_pos_of_level_in_trail_imp M\<^sub>0 lev;
-    ASSERT((n - pos) \<le> uint32_max);
-    ASSERT(n \<ge> pos);
-    let target = n - pos;
-    (_, M, vm') \<leftarrow>
-       WHILE\<^sub>T\<^bsup>\<lambda>(j, M, vm'). j \<le> target\<^esup>
-         (\<lambda>(j, M, vm). j < target)
-         (\<lambda>(j, M, vm). do {
-            ASSERT(Suc j \<le> uint32_max);
-            ASSERT(case M of (M, _) \<Rightarrow> M \<noteq> []);
-            ASSERT(tl_trailt_tr_no_CS_pre M);
-            let L = atm_of (lit_of_last_trail_pol M);
-            ASSERT(vmtf_unset_pre L vm);
-            RETURN (j + 1, tl_trailt_tr_no_CS M, isa_vmtf_unset L vm)
-         })
-         (0, M\<^sub>0, vm);
-    M \<leftarrow> trail_conv_back_imp lev M;
-    RETURN (M, vm')
-  })\<close>
-
-
-abbreviation find_decomp_w_ns_prop where
-  \<open>find_decomp_w_ns_prop \<A> \<equiv>
-     (\<lambda>(M::(nat, nat) ann_lits) highest _.
-        (\<lambda>(M1, vm). \<exists>K M2. (Decided K # M1, M2) \<in> set (get_all_ann_decomposition M) \<and>
-          get_level M K = Suc highest \<and> vm \<in> vmtf \<A> M1))\<close>
-
-definition find_decomp_w_ns where
-  \<open>find_decomp_w_ns \<A> =
-     (\<lambda>(M::(nat, nat) ann_lits) highest vm.
-        SPEC(find_decomp_w_ns_prop \<A> M highest vm))\<close>
-
-lemma isa_find_decomp_wl_imp_find_decomp_wl_imp:
-  \<open>(uncurry2 isa_find_decomp_wl_imp, uncurry2 (find_decomp_wl_imp \<A>)) \<in>
-     [\<lambda>((M, lev), vm). lev < count_decided M]\<^sub>f trail_pol \<A> \<times>\<^sub>f nat_rel \<times>\<^sub>f (Id \<times>\<^sub>r distinct_atoms_rel \<A>) \<rightarrow>
-     \<langle>trail_pol \<A> \<times>\<^sub>r (Id \<times>\<^sub>r distinct_atoms_rel \<A>)\<rangle>nres_rel\<close>
-proof -
-  have [intro]: \<open>(M', M) \<in> trail_pol \<A> \<Longrightarrow>  (M', M) \<in> trail_pol_no_CS \<A>\<close> for M' M
-    by (auto simp: trail_pol_def trail_pol_no_CS_def control_stack_length_count_dec[symmetric])
-
-  have [refine0]: \<open>((0, trail_pol_conv_to_no_CS x1c, x2c),
-        0, trail_conv_to_no_CS x1a, x2a)
-        \<in> nat_rel \<times>\<^sub>r trail_pol_no_CS \<A> \<times>\<^sub>r (Id \<times>\<^sub>r distinct_atoms_rel \<A>)\<close>
-    if
-      \<open>case y of
-       (x, xa) \<Rightarrow> (case x of (M, lev) \<Rightarrow> \<lambda>_. lev < count_decided M) xa\<close> and
-      \<open>(x, y)
-       \<in> trail_pol \<A> \<times>\<^sub>f nat_rel \<times>\<^sub>f (Id \<times>\<^sub>f distinct_atoms_rel \<A>)\<close> and   \<open>x1 = (x1a, x2)\<close> and
-      \<open>y = (x1, x2a)\<close> and
-      \<open>x1b = (x1c, x2b)\<close> and
-      \<open>x = (x1b, x2c)\<close> and
-      \<open>isa_length_trail_pre (trail_pol_conv_to_no_CS x1c)\<close> and
-      \<open>(pos, posa) \<in> nat_rel\<close> and
-      \<open>length (trail_conv_to_no_CS x1a) - posa \<le> uint32_max\<close> and
-      \<open>isa_length_trail (trail_pol_conv_to_no_CS x1c) - pos \<le> uint32_max\<close> and
-      \<open>case (0, trail_conv_to_no_CS x1a, x2a) of
-       (j, M, vm') \<Rightarrow>
-         j \<le> length (trail_conv_to_no_CS x1a) - posa \<and>
-         M = drop j (trail_conv_to_no_CS x1a) \<and>
-         length (trail_conv_to_no_CS x1a) - posa
-         \<le> length (trail_conv_to_no_CS x1a) \<and>
-         vm' \<in> vmtf \<A> M \<and> literals_are_in_\<L>\<^sub>i\<^sub>n \<A> (lit_of `# mset M)\<close>
-     for x y x1 x1a x2 x2a x1b x1c x2b x2c pos posa
-  proof -
-    show ?thesis
-      supply trail_pol_conv_to_no_CS_def[simp] trail_conv_to_no_CS_def[simp]
-      using that by auto
-  qed
-  have trail_pol_empty: \<open>(([], x2g), M) \<in> trail_pol_no_CS \<A> \<Longrightarrow> M = []\<close> for M x2g
-    by (auto simp: trail_pol_no_CS_def ann_lits_split_reasons_def)
-
-  have isa_vmtf: \<open>(x2c, x2a) \<in> Id \<times>\<^sub>f distinct_atoms_rel \<A> \<Longrightarrow>
-       (((aa, ab, ac, ad, ba), baa, ca), x2e) \<in> Id \<times>\<^sub>f distinct_atoms_rel \<A> \<Longrightarrow>
-       x2e \<in> vmtf \<A> (drop x1d x1a) \<Longrightarrow>
-       ((aa, ab, ac, ad, ba), baa, ca) \<in> isa_vmtf \<A> (drop x1d x1a)\<close>
-       for x y x1 x1a x2 x2a x1b x1c x2b x2c pos posa xa x' x1d x2d x1e x2e x1f x2f
-       x1g x1h x2g x2h aa ab ac ad ba baa ca
-       by (cases x2e)
-        (auto 6 6 simp: isa_vmtf_def Image_iff converse_iff prod_rel_iff
-         intro!: bexI[of _ x2e])
-  have trail_pol_no_CS_last_hd:
-    \<open>((x1h, t), M) \<in> trail_pol_no_CS \<A> \<Longrightarrow> M \<noteq> [] \<Longrightarrow> (last x1h) = lit_of (hd M)\<close>
-    for x1h t M
-    by (auto simp: trail_pol_no_CS_def ann_lits_split_reasons_def last_map last_rev)
-
-  have trail_conv_back: \<open>trail_conv_back_imp x2b x1g
-        \<le> SPEC
-           (\<lambda>c. (c, trail_conv_back x2 x1e)
-                \<in> trail_pol \<A>)\<close>
-    if
-      \<open>case y of (x, xa) \<Rightarrow> (case x of (M, lev) \<Rightarrow> \<lambda>vm. lev < count_decided M) xa\<close> and
-      \<open>(x, y) \<in> trail_pol \<A> \<times>\<^sub>f nat_rel \<times>\<^sub>f (Id \<times>\<^sub>f distinct_atoms_rel \<A>)\<close> and
-      \<open>x1 = (x1a, x2)\<close> and
-      \<open>y = (x1, x2a)\<close> and
-      \<open>x1b = (x1c, x2b)\<close> and
-      \<open>x = (x1b, x2c)\<close> and
-      \<open>isa_length_trail_pre (trail_pol_conv_to_no_CS x1c)\<close> and
-      \<open>(pos, posa) \<in> nat_rel\<close> and
-      \<open>length (trail_conv_to_no_CS x1a) - posa \<le> uint32_max\<close> and
-      \<open>isa_length_trail (trail_pol_conv_to_no_CS x1c) - pos \<le> uint32_max\<close> and
-      \<open>(xa, x') \<in> nat_rel \<times>\<^sub>f (trail_pol_no_CS \<A> \<times>\<^sub>f (Id \<times>\<^sub>f distinct_atoms_rel \<A>))\<close> and
-       \<open>x2d = (x1e, x2e)\<close> and
-      \<open>x' = (x1d, x2d)\<close> and
-      \<open>x2f = (x1g, x2g)\<close> and
-      \<open>xa = (x1f, x2f)\<close> and
-      \<open>x2 = count_decided x1e\<close>
-    for x y x1 x1a x2 x2a x1b x1c x2b x2c pos posa xa x' x1d x2d x1e x2e x1f x2f
-       x1g x2g
-   apply (rule trail_conv_back[THEN fref_to_Down_curry, THEN order_trans])
-   using that by (auto simp: conc_fun_RETURN)
-
-
-  show ?thesis
-    supply trail_pol_conv_to_no_CS_def[simp] trail_conv_to_no_CS_def[simp]
-    unfolding isa_find_decomp_wl_imp_def find_decomp_wl_imp_def uncurry_def
-    apply (intro frefI nres_relI)
-    apply (refine_vcg
-      id_trail_conv_to_no_CS[THEN fref_to_Down, unfolded comp_def]
-      get_pos_of_level_in_trail_imp_get_pos_of_level_in_trail[of \<A>, THEN fref_to_Down_curry])
-    subgoal
-      by (rule isa_length_trail_pre) auto
-    subgoal
-      by (auto simp: get_pos_of_level_in_trail_pre_def)
-    subgoal
-      by auto
-    subgoal
-      by (subst isa_length_trail_length_u_no_CS[THEN fref_to_Down_unRET_Id]) auto
-    subgoal
-      by (subst isa_length_trail_length_u_no_CS[THEN fref_to_Down_unRET_Id]) auto
-    apply (assumption+)[10]
-    subgoal
-      by (subst isa_length_trail_length_u_no_CS[THEN fref_to_Down_unRET_Id]) auto
-    subgoal
-      by (subst isa_length_trail_length_u_no_CS[THEN fref_to_Down_unRET_Id]) auto
-    subgoal
-      by (auto dest!: trail_pol_empty)
-    subgoal
-      by (auto dest!: trail_pol_empty)
-    subgoal for x y x1 x1a x2 x2a x1b x1c x2b x2c pos posa
-      by (rule tl_trailt_tr_no_CS_pre) auto
-    subgoal for x y x1 x1a x2 x2a x1b x1c x2b x2c pos posa xa x' x1d x2d x1e x2e x1f x2f
-       x1g x1h x2g x2h
-       by (cases x1g, cases x2h)
-         (auto intro!: vmtf_unset_pre[of _ _ _ _ _ _ \<A> \<open>drop x1d x1a\<close>] isa_vmtf
-           simp: lit_of_last_trail_pol_def trail_pol_no_CS_last_hd lit_of_hd_trail_def)
-    subgoal
-      by (auto simp: lit_of_last_trail_pol_def trail_pol_no_CS_last_hd lit_of_hd_trail_def
-        intro!: tl_trail_tr_no_CS[THEN fref_to_Down_unRET]
-          isa_vmtf_unset_vmtf_unset[THEN fref_to_Down_unRET_uncurry])
-    apply (rule trail_conv_back; assumption)
-    subgoal
-      by auto
-  done
-qed
-
-
-definition (in -) find_decomp_wl_st :: \<open>nat literal \<Rightarrow> nat twl_st_wl \<Rightarrow> nat twl_st_wl nres\<close> where
-  \<open>find_decomp_wl_st = (\<lambda>L (M, N, D, oth).  do{
-     M' \<leftarrow> find_decomp_wl' M (the D) L;
-    RETURN (M', N, D, oth)
-  })\<close>
-
-definition find_decomp_wl_st_int :: \<open>nat \<Rightarrow> isasat \<Rightarrow> isasat nres\<close> where
-  \<open>find_decomp_wl_st_int = (\<lambda>highest S. do{
-     let M = get_trail_wl_heur S;
-     let vm = get_vmtf_heur S;
-     (M', vm) \<leftarrow> isa_find_decomp_wl_imp M highest vm;
-     let S = set_trail_wl_heur M' S;
-     let S = set_vmtf_wl_heur vm S;
-     RETURN S
-  })\<close>
-
-lemma
-  assumes
-    vm: \<open>vm \<in> vmtf \<A> M\<^sub>0\<close> and
-    lits: \<open>literals_are_in_\<L>\<^sub>i\<^sub>n_trail \<A> M\<^sub>0\<close> and
-    target: \<open>highest < count_decided M\<^sub>0\<close> and
-    n_d: \<open>no_dup M\<^sub>0\<close> and
-    bounded: \<open>isasat_input_bounded \<A>\<close>
-  shows
-    find_decomp_wl_imp_le_find_decomp_wl':
-      \<open>find_decomp_wl_imp \<A> M\<^sub>0 highest vm \<le> find_decomp_w_ns \<A> M\<^sub>0 highest vm\<close>
-     (is ?decomp)
-proof -
-  have length_M0:  \<open>length M\<^sub>0 \<le> uint32_max div 2 + 1\<close>
-    using length_trail_uint32_max_div2[of \<A> M\<^sub>0, OF bounded]
-      n_d literals_are_in_\<L>\<^sub>i\<^sub>n_trail_in_lits_of_l[of \<A>, OF lits]
-    by (auto simp: lits_of_def)
-  have 1: \<open>((count_decided x1g, x1g), count_decided x1, x1) \<in> Id\<close>
-    if \<open>x1g = x1\<close> for x1g x1 :: \<open>(nat, nat) ann_lits\<close>
-    using that by auto
-  have [simp]: \<open>\<exists>M'a. M' @ x2g = M'a @ tl x2g\<close> for M' x2g :: \<open>(nat, nat) ann_lits\<close>
-    by (rule exI[of _ \<open>M' @ (if x2g = [] then [] else [hd x2g])\<close>]) auto
-  have butlast_nil_iff: \<open>butlast xs = [] \<longleftrightarrow> xs = [] \<or> (\<exists>a. xs = [a])\<close> for xs :: \<open>(nat, nat) ann_lits\<close>
-    by (cases xs) auto
-  have butlast1: \<open>tl x2g = drop (Suc (length x1) - length x2g) x1\<close> (is \<open>?G1\<close>)
-    if \<open>x2g = drop (length x1 - length x2g) x1\<close> for x2g x1 :: \<open>'a list\<close>
-  proof -
-    have [simp]: \<open>Suc (length x1 - length x2g) = Suc (length x1) - length x2g\<close>
-      by (metis Suc_diff_le diff_le_mono2 diff_zero length_drop that zero_le)
-    show ?G1
-      by (subst that) (auto simp: butlast_conv_take tl_drop_def)[]
-  qed
-  have butlast2: \<open>tl x2g = drop (length x1 - (length x2g - Suc 0)) x1\<close> (is \<open>?G2\<close>)
-    if \<open>x2g = drop (length x1 - length x2g) x1\<close> and x2g: \<open>x2g \<noteq> []\<close> for x2g x1 :: \<open>'a list\<close>
-  proof -
-    have [simp]: \<open>Suc (length x1 - length x2g) = Suc (length x1) - length x2g\<close>
-      by (metis Suc_diff_le diff_le_mono2 diff_zero length_drop that(1) zero_le)
-    have [simp]: \<open>Suc (length x1) - length x2g = length x1 - (length x2g - Suc 0)\<close>
-      using x2g by auto
-    show ?G2
-      by (subst that) (auto simp: butlast_conv_take tl_drop_def)[]
-  qed
-  note butlast = butlast1 butlast2
-
-  have count_decided_not_Nil[simp]:  \<open>0 < count_decided M \<Longrightarrow> M \<noteq> []\<close> for M :: \<open>(nat, nat) ann_lits\<close>
-    by auto
-  have get_lev_last: \<open>get_level (M' @ M) (lit_of (last M')) = Suc (count_decided M)\<close>
-    if \<open>M\<^sub>0 = M' @ M\<close> and \<open>M' \<noteq> []\<close> and \<open>is_decided (last M')\<close> for M' M
-    apply (cases M' rule: rev_cases)
-    using that apply (solves simp)
-    using n_d that by auto
-
-  have atm_of_N:
-    \<open>literals_are_in_\<L>\<^sub>i\<^sub>n \<A> (lit_of `# mset aa) \<Longrightarrow> aa \<noteq> [] \<Longrightarrow> atm_of (lit_of (hd aa)) \<in> atms_of (\<L>\<^sub>a\<^sub>l\<^sub>l \<A>)\<close>
-    for aa
-    by (cases aa) (auto simp: literals_are_in_\<L>\<^sub>i\<^sub>n_add_mset in_\<L>\<^sub>a\<^sub>l\<^sub>l_atm_of_in_atms_of_iff)
-  have Lin_drop_tl: \<open>literals_are_in_\<L>\<^sub>i\<^sub>n \<A> (lit_of `# mset (drop b M\<^sub>0)) \<Longrightarrow>
-      literals_are_in_\<L>\<^sub>i\<^sub>n \<A> (lit_of `# mset (tl (drop b M\<^sub>0)))\<close> for b
-    apply (rule literals_are_in_\<L>\<^sub>i\<^sub>n_mono)
-     apply assumption
-    by (cases \<open>drop b M\<^sub>0\<close>) auto
-
-  have highest: \<open>highest = count_decided M\<close> and
-     ex_decomp: \<open>\<exists>K M2.
-       (Decided K # M, M2)
-       \<in> set (get_all_ann_decomposition M\<^sub>0) \<and>
-       get_level M\<^sub>0 K = Suc highest \<and> vm \<in> vmtf \<A> M\<close>
-    if
-      pos: \<open>pos < length M\<^sub>0 \<and> is_decided (rev M\<^sub>0 ! pos) \<and> get_level M\<^sub>0 (lit_of (rev M\<^sub>0 ! pos)) =
-         highest + 1\<close> and
-      \<open>length M\<^sub>0 - pos \<le> uint32_max\<close> and
-      inv: \<open>case s of (j, M, vm') \<Rightarrow>
-         j \<le> length M\<^sub>0 - pos \<and>
-         M = drop j M\<^sub>0 \<and>
-         length M\<^sub>0 - pos \<le> length M\<^sub>0 \<and>
-         vm' \<in> vmtf \<A> M \<and>
-         literals_are_in_\<L>\<^sub>i\<^sub>n \<A> (lit_of `# mset M)\<close> and
-      cond: \<open>\<not> (case s of
-         (j, M, vm) \<Rightarrow> j < length M\<^sub>0 - pos)\<close> and
-      s: \<open>s = (j, s')\<close> \<open>s' = (M, vm)\<close>
-    for pos s j s' M vm
-  proof -
-    have
-      \<open>j = length M\<^sub>0 - pos\<close> and
-      M: \<open>M = drop (length M\<^sub>0 - pos) M\<^sub>0\<close> and
-      vm: \<open>vm \<in> vmtf \<A> (drop (length M\<^sub>0 - pos) M\<^sub>0)\<close> and
-      \<open>literals_are_in_\<L>\<^sub>i\<^sub>n \<A> (lit_of `# mset (drop (length M\<^sub>0 - pos) M\<^sub>0))\<close>
-      using cond inv unfolding s
-      by auto
-    define M2 and L where \<open>M2 = take (length M\<^sub>0 - Suc pos) M\<^sub>0\<close> and \<open>L = rev M\<^sub>0 ! pos\<close>
-    have le_Suc_pos: \<open>length M\<^sub>0 - pos = Suc (length M\<^sub>0 - Suc pos)\<close>
-      using pos by auto
-    have 1: \<open>take (length M\<^sub>0 - pos) M\<^sub>0 = take (length M\<^sub>0 - Suc pos) M\<^sub>0 @ [rev M\<^sub>0 ! pos]\<close>
-      unfolding le_Suc_pos
-      apply (subst take_Suc_conv_app_nth)
-      using pos by (auto simp: rev_nth)
-    have M\<^sub>0: \<open>M\<^sub>0 = M2 @ L # M\<close>
-      apply (subst append_take_drop_id[symmetric, of _ \<open>length M\<^sub>0 - pos\<close>])
-      unfolding M L_def M2_def 1
-      by auto
-    have L': \<open>Decided (lit_of L) = L\<close>
-      using pos unfolding L_def[symmetric] by (cases L) auto
-    then have M\<^sub>0': \<open>M\<^sub>0 = M2 @ Decided (lit_of L) # M\<close>
-      unfolding M\<^sub>0 by auto
-
-    have \<open>highest = count_decided M\<close> and \<open>get_level M\<^sub>0 (lit_of L) = Suc highest\<close> and \<open>is_decided L\<close>
-      using n_d pos unfolding L_def[symmetric] unfolding M\<^sub>0
-      by (auto simp: get_level_append_if split: if_splits)
-    then show
-     \<open>\<exists>K M2.
-       (Decided K # M, M2)
-       \<in> set (get_all_ann_decomposition M\<^sub>0) \<and>
-       get_level M\<^sub>0 K = Suc highest \<and> vm \<in> vmtf \<A> M\<close>
-      using get_all_ann_decomposition_ex[of \<open>lit_of L\<close> M M2] vm unfolding M\<^sub>0'[symmetric] M[symmetric]
-      by blast
-    show \<open>highest = count_decided M\<close>
-      using  \<open>highest = count_decided M\<close> .
-  qed
-  show ?decomp
-    unfolding find_decomp_wl_imp_def Let_def find_decomp_w_ns_def trail_conv_to_no_CS_def
-      get_pos_of_level_in_trail_def trail_conv_back_def
-    apply (refine_vcg 1 WHILEIT_rule[where R=\<open>measure (\<lambda>(_, M, _). length M)\<close>])
-    subgoal using length_M0 unfolding uint32_max_def by simp
-    subgoal by auto
-    subgoal by auto
-    subgoal using target by (auto simp: count_decided_ge_get_maximum_level)
-    subgoal by auto
-    subgoal by auto
-    subgoal using vm by auto
-    subgoal using lits unfolding literals_are_in_\<L>\<^sub>i\<^sub>n_trail_lit_of_mset by auto
-    subgoal for target s j b M vm by simp
-    subgoal using length_M0 unfolding uint32_max_def by simp
-    subgoal for x s a ab aa bb
-      by (cases \<open>drop a M\<^sub>0\<close>)
-        (auto simp: lit_of_hd_trail_def literals_are_in_\<L>\<^sub>i\<^sub>n_add_mset)
-    subgoal by auto
-    subgoal by (auto simp: drop_Suc drop_tl)
-    subgoal by auto
-    subgoal for s a b aa ba vm x2 x1a x2a
-      by (cases vm)
-        (auto intro!: vmtf_unset_vmtf_tl atm_of_N drop_tl simp: lit_of_hd_trail_def)
-    subgoal for s a b aa ba x1 x2 x1a x2a
-      using lits by (auto intro: Lin_drop_tl)
-    subgoal by auto
-    subgoal by (rule highest)
-    subgoal by (rule ex_decomp) (assumption+, auto)
-    done
-qed
-
-
-lemma find_decomp_wl_imp_find_decomp_wl':
-  \<open>(uncurry2 (find_decomp_wl_imp \<A>), uncurry2 (find_decomp_w_ns \<A>)) \<in>
-    [find_decomp_w_ns_pre \<A>]\<^sub>f Id \<times>\<^sub>f Id \<times>\<^sub>f Id \<rightarrow> \<langle>Id \<times>\<^sub>f Id\<rangle>nres_rel\<close>
-  by (intro frefI nres_relI)
-   (auto simp: find_decomp_w_ns_pre_def simp del: twl_st_of_wl.simps
-       intro!: find_decomp_wl_imp_le_find_decomp_wl')
-
-lemma find_decomp_wl_imp_code_conbine_cond:
-  \<open>(\<lambda>((b, a), c). find_decomp_w_ns_pre \<A> ((b, a), c) \<and> a < count_decided b) = (\<lambda>((b, a), c).
-         find_decomp_w_ns_pre \<A> ((b, a), c))\<close>
-  by (auto intro!: ext simp: find_decomp_w_ns_pre_def)
 
 end
 
