Weidenbach_Book/IsaSAT/IsaSAT_Bump_Heuristics_State.thy
@@ -1,0 +1,91 @@
+theory IsaSAT_Bump_Heuristics_State
+imports Watched_Literals_VMTF
+  IsaSAT_VSIDS
+  Tuple4
+begin
+
+(*TODO: share the to_remove part of Bump_Heuristics*)
+type_synonym bump_heuristics = \<open>(vmtf_remove_int, vmtf_remove_int, bool, nat) tuple4\<close>
+
+abbreviation Bump_Heuristics :: \<open>_ \<Rightarrow> _ \<Rightarrow> _ \<Rightarrow> _ \<Rightarrow> bump_heuristics\<close> where
+  \<open>Bump_Heuristics a b c d \<equiv> Tuple4 a b c d\<close>
+
+lemmas bump_heuristics_splits = Tuple4.tuple4.splits
+hide_fact tuple4.splits
+
+abbreviation get_stable_heuristics :: \<open>bump_heuristics \<Rightarrow> vmtf_remove_int\<close> where
+  \<open>get_stable_heuristics \<equiv> Tuple4_a\<close>
+
+abbreviation get_focused_heuristics :: \<open>bump_heuristics \<Rightarrow> vmtf_remove_int\<close> where
+  \<open>get_focused_heuristics \<equiv> Tuple4_b\<close>
+
+abbreviation is_focused_heuristics :: \<open>bump_heuristics \<Rightarrow> bool\<close> where
+  \<open>is_focused_heuristics \<equiv> Tuple4_c\<close>
+
+abbreviation conflict_count :: \<open>bump_heuristics \<Rightarrow> nat\<close> where
+  \<open>conflict_count \<equiv> Tuple4_d\<close>
+
+abbreviation set_stable_heuristics :: \<open>vmtf_remove_int \<Rightarrow>bump_heuristics \<Rightarrow> _\<close> where
+  \<open>set_stable_heuristics \<equiv> Tuple4.set_a\<close>
+
+abbreviation set_focused_heuristics :: \<open>vmtf_remove_int \<Rightarrow>bump_heuristics \<Rightarrow> _\<close> where
+  \<open>set_focused_heuristics \<equiv> Tuple4.set_b\<close>
+
+abbreviation set_is_focused_heuristics :: \<open>bool \<Rightarrow>bump_heuristics \<Rightarrow> _\<close> where
+  \<open>set_is_focused_heuristics \<equiv> Tuple4.set_c\<close>
+
+abbreviation set_conflict_count :: \<open>nat \<Rightarrow>bump_heuristics \<Rightarrow> _\<close> where
+  \<open>set_conflict_count \<equiv> Tuple4.set_d\<close>
+
+definition bump_heur :: \<open>_ \<Rightarrow> _ \<Rightarrow> bump_heuristics set\<close> where
+  \<open>bump_heur \<A> M = {x.
+    is_focused_heuristics x \<longrightarrow>
+      (get_stable_heuristics x \<in> vmtf \<A> M \<and>
+      get_focused_heuristics x \<in> vmtf \<A> (takeWhile (\<lambda>x. \<not>is_decided x) M)) \<and>
+    \<not>is_focused_heuristics x \<longrightarrow>
+      (get_stable_heuristics x \<in> vmtf \<A> (takeWhile (\<lambda>x. \<not>is_decided x) M) \<and>
+      get_focused_heuristics x \<in> vmtf \<A> M)}\<close>
+
+definition switch_bump_heur :: \<open>bump_heuristics \<Rightarrow> bump_heuristics\<close> where
+  \<open>switch_bump_heur x = do {
+    (set_is_focused_heuristics (\<not>(is_focused_heuristics x)) x)
+  }\<close>
+
+lemma switch_bump_heur:
+  assumes \<open>x \<in> bump_heur \<A> M\<close> and
+    \<open>count_decided M = 0\<close>
+  shows \<open>switch_bump_heur x \<in> bump_heur \<A> M\<close>
+  using assms
+  by (cases x)
+   (auto simp: switch_bump_heur_def bump_heur_def)
+
+
+subsection \<open>Access Function\<close>
+definition isa_vmtf_unset :: \<open>nat \<Rightarrow> bump_heuristics \<Rightarrow> bump_heuristics\<close> where
+  \<open>isa_vmtf_unset L vm = (case vm of Tuple4 (hstable) (focused) foc a \<Rightarrow>
+  Tuple4 (if \<not>foc then vmtf_unset L hstable else hstable)
+    (if foc then vmtf_unset L focused else focused)
+    foc a)\<close>
+
+lemma isa_vmtf_consD:
+  \<open>x \<in> bump_heur \<A> M \<Longrightarrow> x \<in> bump_heur \<A> (L # M)\<close>
+  by (auto simp: bump_heur_def dest: vmtf_consD)
+
+
+lemma isa_vmtf_unset_vmtf_tl:
+  fixes M
+  defines [simp]: \<open>L \<equiv> atm_of (lit_of (hd M))\<close>
+  assumes vmtf:\<open>x\<in> bump_heur \<A> M\<close> and
+    L_N: \<open>L \<in> atms_of (\<L>\<^sub>a\<^sub>l\<^sub>l \<A>)\<close> and [simp]: \<open>M \<noteq> []\<close>
+  shows \<open>isa_vmtf_unset L x \<in> bump_heur \<A> (tl M)\<close>
+proof -
+  obtain ns m fst_As lst_As next_search remove where
+    \<open>is_focused_heuristics x \<Longrightarrow> get_focused_heuristics x = ((ns, m, fst_As, lst_As, next_search), remove)\<close>
+    \<open>\<not>is_focused_heuristics x \<Longrightarrow> get_stable_heuristics x = ((ns, m, fst_As, lst_As, next_search), remove)\<close>
+   by (cases \<open>get_focused_heuristics x\<close>; cases \<open>get_stable_heuristics x\<close>; cases \<open>is_focused_heuristics x\<close>) auto
+  show ?thesis
+    using vmtf_unset_vmtf_tl[of ns m fst_As lst_As next_search remove \<A> M]
+      assms by (auto simp: bump_heur_def)
+qed
+
+end
