Weidenbach_Book/IsaSAT/IsaSAT_VMTF_LLVM.thy
@@ -568,7 +568,7 @@ schematic_goal mk_free_vmtf_remove_assn[sepref_frame_free_rules]: \<open>MK_FREE
   unfolding vmtf_remove_assn_def
   by synthesize_free
 
-definition recombine_vmtf :: \<open>isa_vmtf_remove_int \<Rightarrow> _\<close> where
+definition recombine_vmtf :: \<open>bump_heuristics \<Rightarrow> _\<close> where
   \<open>recombine_vmtf = (\<lambda>x. x)\<close>
 sepref_def recombine_vmtf_impl
    is \<open>RETURN o recombine_vmtf\<close>
@@ -576,7 +576,7 @@ sepref_def recombine_vmtf_impl
    unfolding vmtf_remove_assn_def recombine_vmtf_def
   by sepref
 
-definition split_vmtf :: \<open>isa_vmtf_remove_int \<Rightarrow> _\<close> where
+definition split_vmtf :: \<open>bump_heuristics \<Rightarrow> _\<close> where
   \<open>split_vmtf = (\<lambda>x. x)\<close>
 
 sepref_def split_vmtf_impl
